common/MemoryExplore.v
@@ -1,0 +1,203 @@
+Require Import Zwf.
+Require Import Axioms.
+Require Import CoqlibC.
+Require Intv.
+Require Import MapsC.
+Require Archi.
+Require Import ASTC.
+Require Import Integers.
+Require Import Floats.
+Require Import ValuesC.
+Require Export Memdata.
+Require Export Memtype.
+Require Import sflib.
+Require Import Lia.
+Require Import MemoryC.
+
+Require Import Events.
+Import Mem.
+Local Notation "a # b" := (PMap.get b a) (at level 1).
+
+Local Existing Instance Val.mi_normal.
+
+Inductive mvs_lessdef (chunk: memory_chunk): list memval -> list memval -> Prop :=
+| mvs_lessdef_eq
+    mvs
+  :
+    mvs_lessdef chunk mvs mvs
+| mvs_lessdef_broken
+    mvs
+  :
+    mvs_lessdef chunk (list_repeat (size_chunk_nat chunk) Undef) mvs
+| mvs_lessdef_undef
+    mvs
+  :
+    mvs_lessdef chunk (inj_value chunk.(quantity_chunk) Vundef) mvs
+  (* mvs_lessdef Many32 *)
+  (* [Fragment Vundef Q32 3; Fragment Vundef Q32 2; Fragment Vundef Q32 1; Fragment Vundef Q32 0] *)
+  (* [Byte i; Byte i0; Byte i1; Byte i2] *)
+.
+
+Lemma encode_decode_val
+      chunk mvs
+      (LENGTH: length mvs = (size_chunk_nat chunk))
+  :
+    mvs_lessdef chunk (encode_val chunk (decode_val chunk mvs)) mvs
+.
+Proof.
+  pose chunk.
+  unfold size_chunk_nat, nat_of_Z, size_chunk in *.
+  destruct (proj_bytes mvs) eqn:T; cycle 1.
+  { admit "one case does not hold - Fragment - Byte ". }
+(* { unfold encode_val, decode_val. *)
+(*     Ltac des_nat := match goal with *)
+(*                     | [n: nat |- _] => destruct n; ss *)
+(*                     end. *)
+(*     Ltac des_outest_if := *)
+(*       match goal with *)
+(*       | [ H: context[match ?X with _ => _ end] |- _ ] => let name := fresh "NAME" in destruct X eqn:NAME *)
+(*       end. *)
+(*     Ltac simpl_true := *)
+(*       match goal with *)
+(*       | [ H: ?b0 && ?b1 = true |- _ ] => apply andb_true_iff in H; des *)
+(*       end. *)
+(*     des_ifs; ss; des_ifs; ss; try (econsby ss); *)
+(*       unfold proj_value in *; des_ifs; ss. *)
+(*     - repeat (des_outest_if; repeat (simpl_true); des_sumbool; clarify). econs; eauto. *)
+(*     - repeat (des_outest_if; repeat (simpl_true); des_sumbool; clarify). econs; eauto. *)
+(*     - repeat (des_outest_if; repeat (simpl_true); des_sumbool; clarify). *)
+(* (* mvs_lessdef Mint64 (inj_bytes (encode_int 8 (Int64.unsigned i))) *) *)
+(* (*   [Fragment (Vlong i) Q64 7; Fragment (Vlong i) Q64 6; Fragment (Vlong i) Q64 5; Fragment (Vlong i) Q64 4; *) *)
+(* (*   Fragment (Vlong i) Q64 3; Fragment (Vlong i) Q64 2; Fragment (Vlong i) Q64 1; Fragment (Vlong i) Q64 0] *) *)
+(*       admit "raw admit!!!!!!!!!!!!!!!!!!!!!!". *)
+(*     - repeat (des_outest_if; repeat (simpl_true); des_sumbool; clarify). econs; eauto. *)
+(*     - repeat (des_outest_if; repeat (simpl_true); des_sumbool; clarify). econs; eauto. *)
+(*     - repeat (des_outest_if; repeat (simpl_true); des_sumbool; clarify). econs; eauto. *)
+(*     - repeat (des_outest_if; repeat (simpl_true); des_sumbool; clarify). econs; eauto. *)
+(*     - repeat (des_outest_if; repeat (simpl_true); des_sumbool; clarify). econs; eauto. *)
+(*     - repeat (des_outest_if; repeat (simpl_true); des_sumbool; clarify). econs; eauto. *)
+(*   } *)
+  
+  exploit inj_proj_bytes; eauto. i; clarify.
+  exploit length_proj_bytes; eauto. i; clarify.
+
+  unfold encode_val, decode_val.
+  Ltac des_list := match goal with
+                   | [l: list byte |- _] => destruct l; ss
+                   end.
+  unfold inj_bytes in *.
+  des_ifs; ss; try (econsby ss).
+  - repeat (des_list; des_ifs; ss; []).
+    admit "maybe true".
+  - repeat (des_list; des_ifs; ss; []).
+    admit "maybe true".
+  - repeat (des_list; des_ifs; ss; []).
+    admit "maybe true".
+  - repeat (des_list; des_ifs; ss; []).
+    admit "maybe true".
+  - repeat (des_list; des_ifs; ss; []).
+    admit "maybe true".
+  - repeat (des_list; des_ifs; ss; []).
+    admit "maybe true".
+  - repeat (des_list; des_ifs; ss; []).
+    admit "maybe true".
+  - repeat (des_list; des_ifs; ss; []).
+    admit "maybe true".
+Qed.
+
+Local Transparent Mem.store Mem.load.
+Lemma Mem_load_store_extends
+      m0 m1 chunk blk ofs v
+      (LOAD: Mem.load chunk m0 blk ofs = Some v)
+      (STORE: Mem.store chunk m0 blk ofs v = Some m1)
+  :
+    Mem.extends m1 m0
+.
+Proof.
+  hexploit Mem_store_perm_iff; eauto. intro PERM.
+  (* unfold load, store in *; ss. des_ifs; ss. *)
+
+  assert(TY: Val.has_type v (type_of_chunk chunk)).
+  { eapply Mem.load_type; eauto. }
+  econs; eauto with mem.
+  unfold inject_id.
+  econs; ii; ss; clarify; eauto.
+  - rewrite Z.add_0_r. eapply PERM; eauto.
+  - apply Z.divide_0_r.
+  - rewrite Z.add_0_r. apply PERM in H0. clear PERM.
+    unfold load in *. des_ifs.
+    unfold store in *. des_ifs; ss.
+    rewrite PMap.gsspec. des_ifs; cycle 1.
+    { destruct (ZMap.get ofs0 (mem_contents m0) # b2) eqn:T; econs; ss; eauto.
+      apply val_inject_id. econs; eauto. }
+    destruct (classic (ofs <= ofs0 < ofs +
+Z.of_nat (length (encode_val chunk (decode_val chunk (getN (size_chunk_nat chunk) ofs (mem_contents m0) # blk)))))); cycle 1.
+    { erewrite setN_outside; try xomega.
+      destruct (ZMap.get ofs0 (mem_contents m0) # blk) eqn:T; econs; ss; eauto.
+      apply val_inject_id. econs; eauto.
+    }
+    hexploit setN_in; eauto. instantiate (1:= (mem_contents m0) # blk).
+    rewrite ! encode_val_length in *; rewrite <- ! size_chunk_conv in *.
+    intro IN.
+    set (encode_val chunk (decode_val chunk (getN (size_chunk_nat chunk) ofs (mem_contents m0) # blk)))
+      as newv in *.
+    set ((mem_contents m0) # blk) as contents in *.
+    (* We should change memval_inject!!!!
+  mvs_lessdef Many32
+  [Fragment Vundef Q32 3; Fragment Vundef Q32 2; Fragment Vundef Q32 1; Fragment Vundef Q32 0]
+  [Byte i; Byte i0; Byte i1; Byte i2]
+
+mvs_lessdef Mint64 (inj_bytes (encode_int 8 (Int64.unsigned i)))
+  [Fragment (Vlong i) Q64 7; Fragment (Vlong i) Q64 6; Fragment (Vlong i) Q64 5; Fragment (Vlong i) Q64 4;
+  Fragment (Vlong i) Q64 3; Fragment (Vlong i) Q64 2; Fragment (Vlong i) Q64 1; Fragment (Vlong i) Q64 0]
+*)
+Abort.
+Local Opaque Mem.store Mem.load.
+
+(* m0 -store v-> m1 // m0 -load v-> m1' ===> m1' is better state than m1. (load is harder than store) *)
+(* this should hold *)
+Lemma Mem_store_left_inject
+      j0 m_src0 m_src1 m_tgt
+      (INJ: Mem.inject j0 m_src0 m_tgt)
+      v_src v_tgt
+      (INJV: Val.inject j0 v_src v_tgt) 
+      ty rsp_src rsp_tgt rspdelta ofs
+      (SRC: Mem.storev (chunk_of_type ty) m_src0 (Vptr rsp_src ofs true) v_src = Some m_src1)
+      (TGT: Mem.loadv (chunk_of_type ty) m_tgt (Vptr rsp_tgt (Ptrofs.add ofs rspdelta) true) = Some v_tgt)
+      (INJRSP: j0 rsp_src = Some (rsp_tgt, rspdelta.(Ptrofs.unsigned)))
+  :
+    <<INJ: Mem.inject j0 m_src1 m_tgt>>
+.
+Proof.
+  unfold storev in *. des_ifs. ss.
+  hexploit Mem_store_perm_eq; eauto. intro PERM.
+
+  exploit store_mapped_inject; eauto. intro STORETGT; des.
+  eapply inject_extends_compose; eauto.
+  eapply Mem_load_store_extends; eauto.
+  rpapply STORETGT. f_equal.
+  rewrite Ptrofs.add_unsigned. rewrite Ptrofs.unsigned_repr; ss.
+  admit "sz".
+  Ptrofs.repr_unsigned:
+  ss.
+  { unfold loadv.
+  eapply extends_inject_compose; eauto.
+  assert(n2 = m_tgt).
+  { clear - STORETGT TGT. admit "". }
+  clarify.
+
+  econs; try apply INJ; eauto.
+  - econs; ii; try eapply INJ; ii; eauto with mem congruence.
+    Local Transparent Mem.store. unfold Mem.store in *. des_ifs; ss.
+    rewrite PMap.gsspec. des_ifs.
+    + Local Transparent Mem.load. unfold Mem.load in *. des_ifs; ss.
+      destruct (classic
+                  (Ptrofs.unsigned ofs <= ofs0 <
+                   Ptrofs.unsigned ofs + Z.of_nat (length (encode_val (chunk_of_type ty) v_src)))); cycle 1.
+      { rewrite setN_outside; try omega. eapply INJ; eauto. }
+      clear - INJV H H1. abstr (chunk_of_type ty) chnk.
+      admit "this should hold".
+Admitted.
+
+
+End ARGPASSING.
